coq/cclc/clc_typing.v
@@ -39,15 +39,15 @@ Inductive clc_type : context term -> term -> term -> sort -> Prop :=
 | clc_it Γ :
   Γ |> U ->
   Γ ⊢ It : Unit : U
-| clc_bool Γ :
+| clc_either Γ :
   Γ |> U ->
-  Γ ⊢ Bool : U @ 0 : U
+  Γ ⊢ Either : U @ 0 : U
 | clc_left Γ :
   Γ |> U ->
-  Γ ⊢ Left : Bool : U
+  Γ ⊢ Left : Either : U
 | clc_right Γ :
   Γ |> U ->
-  Γ ⊢ Right : Bool : U
+  Γ ⊢ Right : Either : U
 | clc_sigma Γ A B s r t i :
   s ⋅ r ≤ t ->
   Γ |> U ->
@@ -65,8 +65,8 @@ Inductive clc_type : context term -> term -> term -> sort -> Prop :=
 | clc_case Γ1 Γ2 Γ m n1 n2 A s t i :
   Γ1 |> s ->
   Γ1 ∘ Γ2 => Γ ->
-  Γ1 ⊢ m : Bool : U ->
-  [Bool :{s} Γ2] ⊢ A : t @ i : U ->
+  Γ1 ⊢ m : Either : U ->
+  [Either :{s} Γ2] ⊢ A : t @ i : U ->
   Γ2 ⊢ n1 : A.[Left/] : t ->
   Γ2 ⊢ n2 : A.[Right/] : t ->
   Γ ⊢ Case m n1 n2 : A.[m/] : t
